{
 "cells": [
  {
   "cell_type": "markdown",
   "metadata": {},
   "source": [
    "## Problem 2\n",
    "\n",
    "### Part A\n",
    "<body>\n",
    "   Show that $ argmin(\\beta) : \\frac{1}{n} \\sum_i^n(x_i \\beta - y_i)^2 $ has form:\n",
    "      <p>$$ A\\beta^{2} + B\\beta + C $$</p>\n",
    "   \n",
    "   First we expand:\n",
    "      <p>$$\\frac{1}{n} [\\sum_i^n((x_i\\beta)^2-2x_iy_i\\beta + y_{i}^{2})]$$</p>\n",
    "   Moving the sum inside:   \n",
    "      <p>$$\\Rightarrow (\\frac{1}{n}\\sum_i^n x_i^2)\\beta^2 + (\\frac{-2}{n}\\sum_i^nx_iy_i)\\beta + (\\frac{1}{n}\\sum_i^n y_i^2)$$</p>\n",
    "\n",
    "   Now we can see that:\n",
    "      <p>$$A(x_i,y_i) = \\frac{1}{n}\\sum_i^n x_i^2$$</p>\n",
    "      <p>$$B(x_i,y_i) = \\frac{-2}{n}\\sum_i^nx_iy_i$$</p>\n",
    "      <p>$$C(x_i,y_i) = \\frac{1}{n}\\sum_i^n y_i^2$$</p>\n",
    "</body>\n",
    "\n",
    "### Part B\n",
    "<body>\n",
    "   To show that A is always positive, we simply observe that $n > 1$, and assuming $x_i \\in \\bf{R}$, any real number times itself is always non-negative. Then a sum of non-negative real numbers is also non-negative. Therefore we cannot have $A < 0$ .\n",
    "</body>\n",
    "\n",
    "### Part C\n",
    "<body>\n",
    "   We take the derivative with respect to $\\beta$ and set the equation equal to zero to find the solution to our original problem, $ argmin(\\beta) : \\frac{1}{n} \\sum_i^n(x_i \\beta - y_i)^2 $.\n",
    "   <p>\n",
    "      $$\\bigtriangledown_{\\beta}[\\frac{1}{n} \\sum_i^n(x_i \\beta - y_i)^2] = 0$$\n",
    "   </p>\n",
    "   <p>\n",
    "      $$\\Rightarrow\\frac{2}{n}\\sum_i^nx_i^2\\beta - \\frac{2}{n}\\sum_i^ns_iy_i = 0$$\n",
    "   </p>\n",
    "   <p>\n",
    "      $$\\Rightarrow\\sum_i^nx_i^2\\beta = \\sum_i^nx_iy_i$$\n",
    "   </p>\n",
    "   <p>\n",
    "      $$\\Rightarrow\\beta = \\sum_i^n(\\frac{x_iy_i}{x_i^2}) = \\frac{\\pmb{x}^T\\cdot\\pmb{y}}{\\|x\\|_2^2}$$\n",
    "   </p>\n",
    "</body>\n",
    "\n",
    "### Part D\n",
    "<body>\n",
    "   <p>\n",
    "        Now we assume some error vector $\\pmb{e}$ ($\\pmb{e} = (e_1, e_2, ... , e_n)$), and find out what our new $\\beta$ is (denoted by $\\hat{\\beta}$).\n",
    "   </p>\n",
    "   <p>\n",
    "       We are given that $\\hat{\\beta} = \\beta + \\pmb{Z}\\pmb{e}$ and that $y_i^{*} = x_i\\beta + e_i$. We plug in $y_i^{*}$ to $\\beta$ and solve for $\\hat{\\beta}$ .\n",
    "   <p>\n",
    "      $$\\Rightarrow \\hat{\\beta} = \\sum_i^n\\frac{x_i(x_i\\beta + e_i)}{x_i^2} = \\sum_i^n\\frac{x_i}{x_i}\\beta + \\sum_i^n\\frac{x_i e_i}{x_i^2}$$\n",
    "   </p>\n",
    "   <p>\n",
    "      $$\\Rightarrow \\hat{\\beta} = \\beta + \\sum_i^n\\frac{1}{x_i}e_i$$\n",
    "   </p>\n",
    "   <p>\n",
    "      $$\\Rightarrow \\hat{\\beta} = \\beta + \\frac{\\pmb{x}}{\\pmb{x}^T\\pmb{x}}\\pmb{e}$$\n",
    "   </p>\n",
    "\n",
    "   <p>\n",
    "      $$\\vec{z} = \\frac{\\pmb{x}}{\\|\\pmb{x}\\|_2^2} $$\n",
    "   </p>\n",
    "\n",
    "</body>\n",
    "\n",
    "### Bonus\n",
    "<body>\n",
    "   <p>\n",
    "      In the general case, we have:\n",
    "   </p>\n",
    "   <p>\n",
    "      $$\\bigtriangledown_\\beta\\,\\, \\frac{1}{n} \\|\\hat{\\pmb{y}}\\,\\, -\\,\\, \\pmb{y}\\|_2^2 \\,\\,=\\,\\, 0$$\n",
    "   </p>\n",
    "   <p>\n",
    "      $$\\Rightarrow\\frac{1}{n} \\bigtriangledown_\\beta\\,\\, \\|\\pmb{X}\\beta \\,\\,-\\,\\, \\pmb{y}\\|_2^2\\,\\, = \\,\\,0$$\n",
    "   </p>\n",
    "   <p>\n",
    "      $$\\Rightarrow \\bigtriangledown_\\beta \\,\\,(\\pmb{X}\\beta - \\pmb{y})^{T})\\,(\\pmb{X}\\beta - \\pmb{y})\\,\\, =\\,\\, 0$$\n",
    "   </p>\n",
    "   <p>\n",
    "      $$\\Rightarrow \\bigtriangledown_\\beta \\,\\,(\\beta^T\\pmb{X}^T\\pmb{X}\\beta\\,\\, -\\,\\, 2\\beta^T\\pmb{X}^T\\pmb{y}\\,\\, + \\,\\,\\pmb{y}^T\\pmb{y})\\,\\, =\\,\\, 0$$\n",
    "   </p>\n",
    "   <p>\n",
    "      $$\\Rightarrow \\,\\, 2 \\pmb{X}^T \\pmb{X} \\beta \\,\\, - \\,\\, 2 \\pmb{X}^T \\pmb{y} \\,\\, = \\,\\, 0$$\n",
    "   </p>\n",
    "   <p>\n",
    "      $$\\Rightarrow \\,\\, \\beta \\,\\, = \\,\\, (\\pmb{X}^T \\pmb{X})^{-1} \\, \\pmb{X}^T \\pmb{y}$$\n",
    "   </p>"
   ]
  },
  {
   "cell_type": "code",
   "execution_count": null,
   "metadata": {},
   "outputs": [],
   "source": []
  }
 ],
 "metadata": {
  "kernelspec": {
   "display_name": "Python 3",
   "language": "python",
   "name": "python3"
  },
  "language_info": {
   "codemirror_mode": {
    "name": "ipython",
    "version": 3
   },
   "file_extension": ".py",
   "mimetype": "text/x-python",
   "name": "python",
   "nbconvert_exporter": "python",
   "pygments_lexer": "ipython3",
   "version": "3.5.2"
  }
 },
 "nbformat": 4,
 "nbformat_minor": 2
}
